src/tls/Handshake.fst
@@ -7,6 +7,7 @@ module Handshake
 open TLSExtensions //the other opens are in the .fsti
 open CoreCrypto
 open HSCrypto
+open HandshakeLog
 
 let hsId h = noId // Placeholder
 
@@ -61,7 +62,7 @@ val negotiate:list 'a -> list 'a -> Tot (option 'a)
 let negotiate l1 l2 =
   List.Tot.tryFind (fun s -> List.Tot.existsb (fun c -> c = s) l1) l2
 
-val negotiateCipherSuite: cfg:config -> pv:protocolVersion -> c:known_cipher_suites -> Tot (result (TLSConstants.kexAlg * option TLSConstants.sigAlg * TLSConstants.aeAlg * known_cipher_suite))
+val negotiateCipherSuite: cfg:config -> pv:protocolVersion -> c:valid_cipher_suites -> Tot (result (TLSConstants.kexAlg * option TLSConstants.sigAlg * TLSConstants.aeAlg * valid_cipher_suite))
 let negotiateCipherSuite cfg pv c =
   match negotiate c cfg.ciphersuites with
   | Some(CipherSuite kex sa ae) -> Correct(kex,sa,ae,CipherSuite kex sa ae)
@@ -164,7 +165,7 @@ let acceptableVersion cfg ch s_pv s_random =
   - TODO: [s_cs] is supported by the protocol version (e.g. no GCM with
     TLS<1.2).
 *)
-val acceptableCipherSuite: config -> ch -> protocolVersion -> known_cipher_suite -> Tot bool
+val acceptableCipherSuite: config -> ch -> protocolVersion -> valid_cipher_suite -> Tot bool
 let acceptableCipherSuite cfg ch s_pv s_cs =
   // JP: I would think the first line implies the second one?
   List.Tot.existsb (fun x -> x = s_cs) ch.ch_cipher_suites &&
